Assignment 2 in Methods: 

Using parts of old assignments from latex. I first converted the assignments to .md and then used parts of them and played with it. I hope it is okay that I do not include all the latex-files I used as a source. I read this option to late.

Question 1 
==========

a
-

<span>eststo: reg lnc lnp lny, cluster(state)</span>\
Results can be seen in Table 1

b 
-

<span>quietly tab year, gen(period)</span>\
<span>eststo: xtreg lnc lnp lny period\*,fe cluster(state)</span>\
<span>eststo: reg d.lnc d.lnp d.lny d.period\*, cluster(state)</span>\
<span>xtserial lnc lnp lny</span>\
$$\begin{align*}
lnC_{it}= \alpha + \beta_{1}lnP_{it} + \beta_{2}lnY_{it} + \gamma_{2} D_{2i}+... + \gamma_{46} D_{46i}+ \delta_{1} T1_{t} + ...+ \delta_{29} T29_{t}+u_{it}\end{align*}$$
In order to account for time effects dummy variables (T1-T29) for each
but one year are included. To include state effects there are several
options. Firstly dummy variables (D2-D46) for each state can be added to
the regression. Equivalently, a fixed effect within transformation can
be applied to get rid of unobserved state-specific effects. If the
state-specific effects can be argued to be uncorrelated with the
included regressors, a random effects model can be estimated. In fact,
the Hausmann test does no reject the RE model. Since the RE model yields
very similar estimates we will stick with the FE model for comparative
purposes.\
\
Given that smoking is an addiction it is plausible that there might be
serial correlation, which is confirmed by a test for serial correlation
in the residuals obtained from the FD regression. Given substantial
serial correlation, the FD regression should generally be preferred.\



e 
-

<span>eststo: xtreg lnc lnp lny period\* gln\*, cluster(state)</span>\
<span>eststo: reg d.lnc d.lnp d.lny d.period\* d.gln\*,
cluster(state)</span>\
As argued in the paper by Baltagi & Li (1999) when modelling the demand
of cigarettes it is appropriate to take into account spatial correlation
across states due to border effect purchases. Further, interaction
between states can result in correlated outcome. Over this suggests that
the error terms are correlated across states. To account for this
correlation amongst states, interaction variables that reflect
endogenous and exogenous interaction effects can be added to the
regression.\
\
Endogenous effects suggest that the demand of a state is influenced by
its neighbours’ outcomes. We are trying to capture this effect by
including $glnc$, which, for each individual state, represents the
average cigarette demand of those other states it is related to as
determined by the matrix $D$. This effect is likely to be endogenous as
there is a feedback process taking place between neighbours, since links
between states should be reciprocal given the spatial weight matrix.
However, only the final outcome of the feedback process will be measured
and it is impossible to differentiate the causal affect of a particular
state $j$ on $i$ and vice versa. In order to make out this causal impact
instrumental variables are a solution. Availability of instrumental
variables is determined by the existence of intransitive triads in the
network structure. As each individual state has its own group that it
interacts with, it should be possible to find a state k that is related
to state j but not i such that $G_{ik}=0$ and $G_{ij} \cdot G_{jk}>0$.
Exogenous characteristics of this state $k$ can then be used as an
instrument for $j$ and thus the causal effect of $j$ on $i$ can be
isolated.\
\
With instrumental variables, it is also possible to differentiate
exogenous from endogenous effects and thus to break the reflection
problem. Exogenous interaction effects refer to correlated outcomes as
$j$’s socioeconomic characteristics impact on $i$’s outcome, vice versa.


Question 2
==========

a
-

$$\begin{align*}
lnC_{it}= \alpha + \beta_{1}lnP_{it} + \beta_{2}lnY_{it} + \gamma_{2} D_{2i}+... + \gamma_{46} D_{46i}+ \delta_{1} T1_{t} + ...+ \delta_{29} T29_{t}+u_{it}\end{align*}$$


$$\begin{align*}
& E[y_{i} | a^{l}_{i}=0, s_{i}=0] = \alpha - \gamma \frac{\pi_{0}}{\pi_{2}}\\
& E[y_{i} | a^{l}_{i}=0, s_{i}=1] = \alpha - \gamma \frac{\pi_{0}}{\pi_{2}} + \beta - \frac{1}{\pi_{2}} (\gamma \pi_{1} + \tau (\pi_{0}+\pi_{1}) ) \\
& E[y_{i} | a^{l}_{i}=1, s_{i}=0] = \alpha - \gamma \frac{\pi_{0}}{\pi_{2}}+\frac{\gamma}{\pi_{2}}\\
& E[y_{i} | a^{l}_{i}=1, s_{i}=1] = \alpha + \beta - \frac{1}{\pi_{2}}(\gamma (\pi_{0}+(\pi_{1}-1)+\tau(\pi_{0}+\pi_{1}-1))\\
\end{align*}$$

b
-

$$\begin{align*}
& E[y_{i} | a^{l}_{i}=0, s_{i}=1] - E[y_{i} | a^{1}_{i}=0, s_{i}=0]  = \beta - \gamma \frac{\pi_{1}}{\pi_{2}}-\frac{\tau}{\pi_{2}}(\pi_{0}+\pi_{1}) \\
& \text{If }\pi_{0} = \pi_{1} = 0, \\
& E[y_{i} | a^{l}_{i}=0, s_{i}=1] - E[y_{i} | a^{1}_{i}=0, s_{i}=0]  = \beta - \gamma \frac{0}{\pi_{2}}-\frac{\tau}{\pi_{2}}(0+0) = \beta \\
\end{align*}$$



Proxy controls partially account for OVB, which is the main reason for
including them in a regression. Yet, they are simultaneously determined
by the regressor of interest. This is also the case in our example where
late ability is causally related to the omitted variable ability, which
is meant to represent, yet it is equally a function of the regressor
high school education. Including proxy controls will thus lead to biased
estimates as highlighted by the equations in part a (though this bias
might be an improvement over the bias present when not at all accounting
for OVB). The restriction suggests that the proxy variable late ability
is neither causally affected by high school education, so it is not
itself an intermediate outcome, nor is it subject to a general shift
which would be reflected in the constant. Instead, this assumption
implies that the proxy variable late ability is purely a function of the
latent variable, ability $a_{i}$, that we are trying to capture with it.
Given this assumption it is possible to identify the direct effect of
completed high school education on future earnings.

$$\begin{align*}
 \text{If }-\frac{\tau}{\gamma}=\frac{\pi_{1}}{\pi_{0}+\pi_{1}} \Rightarrow -\tau = \frac{\gamma \pi_{1}}{\pi_{0}+\pi_{1}} \\
 E(y_{i} | \alpha^{l}_{i} = 0, s_{i} = 1) - E(y_{i} | \alpha^{l}_{i} = 0, s_{i} = 0)
& = \beta - \gamma \frac{\pi_{1}}{\pi_{2}}+ \frac{\gamma \pi_{1}}{\pi_{0}+\pi_{1}} \cdot \frac{\pi_{0}+\pi_{1}}{\pi_{2}}  \\
& = \beta - \gamma \frac{\pi_{1}}{\pi_{2}} + \gamma \frac{\pi_{1}}{\pi_{2}} \\ & = \beta\end{align*}$$

Question 3 - extra
==========
Let's see what nice more math and pictures I can find:

$$\begin{align*}
& max \; u_1(x) \text{ s.t. } p_1 x_1 + p_2 x_2 \le w_1 \\
& L (x_1, x_2, p_1, p_2, w_1) = x_1^{3/4} x_2^{1/4} - \lambda (p_1 x_1 + p_2 x_2 - w_1) \\
&\text{FOC} \\
& \frac{{\partial}L}{{\partial}x_1} =  \frac{3}{4} x_1^{-1/4} x_2^{1/4} - \lambda p_1 = 0 \\
& \frac{{\partial}L}{{\partial}x_2} =  \frac{1}{4} x_1^{3/4} x_2^{-3/4} - \lambda p_2 = 0 \\
& \frac{{\partial}L}{{\partial}x_1} /  \frac{{\partial}L}{{\partial}x_2}: = \frac{ \frac{3}{4} x_1^{-1/4} x_2^{1/4} }{ \frac{1}{4} x_1^{3/4} x_2^{-3/4}} = \frac{ \lambda p_1}{  \lambda p_2} \\
& \iff  3 x_1^{-1} x_2 = \frac{ p_1}{  p_2} \\
& \iff  x_2 = \frac{ x_1 p_1}{ 3 p_2}, \quad x_1 = \frac{  x_2 p_2 3}{   p_1} \\ 
&p_1 x_1 + p_2 x_2 = w_1 \iff p_1 x_1 + p_2 \frac{ x_1 p_1}{ 3 p_2} = w_1 \\
&\iff p_1 x_1 + \frac{ x_1 p_1}{ 3 } = w_1 \\
&\iff x_1( 1 + \frac{ 1}{ 3 }) = \frac{w_1}{p_1} \\
&\iff x_1 = \frac{3 w_1}{4 p_1} = x_{1,1}\text{ , }  (x_{good, consumer})\\\end{align*}$$
$$\begin{align*}
&p_1 x_1 + p_2 x_2 = w_1 \iff p_1 \frac{  x_2 p_2 3}{   p_1} + p_2 x_2 = w_1 \\
& \iff x_2 = \frac{w_1}{4 p_2} = x_{2,1}\text{ , }  (x_{good, consumer})\end{align*}$$

$$\begin{align*}
& max \; u_1(x) \text{ s.t. } p_1 x_1 + p_2 x_2 \le w_1 \\
& L (x_1, x_2, p_1, p_2, w_1) = x_1^{3/4} x_2^{1/4} - \lambda (p_1 x_1 + p_2 x_2 - w_1) \\
&\text{FOC} \\
& \frac{{\partial}L}{{\partial}x_1} =  \frac{3}{4} x_1^{-1/4} x_2^{1/4} - \lambda p_1 = 0 \\
& \frac{{\partial}L}{{\partial}x_2} =  \frac{1}{4} x_1^{3/4} x_2^{-3/4} - \lambda p_2 = 0 \\
& \frac{{\partial}L}{{\partial}x_1} /  \frac{{\partial}L}{{\partial}x_2}: = \frac{ \frac{3}{4} x_1^{-1/4} x_2^{1/4} }{ \frac{1}{4} x_1^{3/4} x_2^{-3/4}} = \frac{ \lambda p_1}{  \lambda p_2} \\
& \iff  3 x_1^{-1} x_2 = \frac{ p_1}{  p_2} \\
& \iff  x_2 = \frac{ x_1 p_1}{ 3 p_2}, \quad x_1 = \frac{  x_2 p_2 3}{   p_1} \\ 
&p_1 x_1 + p_2 x_2 = w_1 \iff p_1 x_1 + p_2 \frac{ x_1 p_1}{ 3 p_2} = w_1 \\
&\iff p_1 x_1 + \frac{ x_1 p_1}{ 3 } = w_1 \\
&\iff x_1( 1 + \frac{ 1}{ 3 }) = \frac{w_1}{p_1} \\
&\iff x_1 = \frac{3 w_1}{4 p_1} = x_{1,1}\text{ , }  (x_{good, consumer})\\\end{align*}$$
$$\begin{align*}
&p_1 x_1 + p_2 x_2 = w_1 \iff p_1 \frac{  x_2 p_2 3}{   p_1} + p_2 x_2 = w_1 \\
& \iff x_2 = \frac{w_1}{4 p_2} = x_{2,1}\text{ , }  (x_{good, consumer})\end{align*}$$

-------------

(i)\
$D_p x_i(p,w_i)$ is negative semidefinite if $x_i(p,w_i)$ satisfies
ULD.\
Hence, if $(p'-p) [x_i(p',w_i) - x_i(p,w_i)] \le 0$, $x_i(p,w_i)$
satisfies ULD.\
Let $(p'-p) = [0,...,0,p'_i - p_i,0,...,0] = dp > 0$ and
$\exists \epsilon, \; dp < \epsilon \; \forall \; \epsilon$.\
Then, we have
$(p'-p) [x_i(p',w_i) - x_i(p,w_i)] = dp' \frac{{\partial}x_i(p, w_i)}{{\partial}p_i} dp \le 0$.\
Hence $D_p x_i(p,w_i)$ is negative semidefinite $\forall p$\
(ii)\
Show that $x_i(p,w_i)$ satisfies the uncompensated law of demand if
$D_p x_i(p,w_i)$ is negative definite $\forall p$.\
Let $p(\lambda) = (1-\lambda) p + \lambda p' > p, \; \lambda \in (0,1)$\

---------

The question ask to transfer initial income, here denoted by the
numeraire $m$, so that the product of the utilities is maximized.
$$\begin{align*}
&\max \Pi_{i=1}^4 u_i \quad s.t. \sum_{i=1}^4 u_i = 130 \\
&L = (m_1 + 2 \cdot 1\sqrt{x_1})(m_2 + 2 \cdot 2\sqrt{x_2})(m_3 + 2 \cdot 3\sqrt{x_3})(m_4 + 2 \cdot 4\sqrt{x_4}) \\ &- \lambda (m_1 + m_2 + m_3 +m_4 - 100) \\
&FOC \text{ (everything with equality because we know that everybody consumes)}: \\
&\frac{{\partial}L}{{\partial}m_1} := (m_2 + 2 \cdot 2\sqrt{x_2})(m_3 + 2 \cdot 3\sqrt{x_3})(m_4 + 2 \cdot 4\sqrt{x_4}) - \lambda = 0 \\
&\frac{{\partial}L}{{\partial}m_2} := (m_1 + 2 \cdot 1\sqrt{x_1})(m_3 + 2 \cdot 3\sqrt{x_3})(m_4 + 2 \cdot 4\sqrt{x_4}) - \lambda = 0 \\
&\frac{{\partial}L}{{\partial}m_3} := (m_2 + 2 \cdot 2\sqrt{x_2})(m_1 + 2 \cdot 1\sqrt{x_1})(m_4 + 2 \cdot 4\sqrt{x_4}) - \lambda = 0 \\
&\frac{{\partial}L}{{\partial}m_4} := (m_2 + 2 \cdot 2\sqrt{x_2})(m_3 + 2 \cdot 3\sqrt{x_3})(m_1 + 2 \cdot 1\sqrt{x_1}) - \lambda = 0 \\
&\frac{{\partial}L}{{\partial}\lambda} := m_1 + m_2 + m_3 +m_4 - 100 = 0 \\
&\frac{{\partial}L / {\partial}m_1}{{\partial}L / {\partial}m_2} = \frac{m_2 + 2 \cdot 2\sqrt{x_2}}{m_1 + 2 \cdot 1\sqrt{x_1}} = 1 \iff m_2 + 2 \cdot 2\sqrt{x_2} = m_1 + 2 \cdot 1\sqrt{x_1}\\
&\text{We further get: } \\
& m_1 + 2 \cdot 1\sqrt{x_1} = m_2 + 2 \cdot 2\sqrt{x_2} = m_3 + 2 \cdot 3\sqrt{x_3} = m_4 + 2 \cdot 4\sqrt{x_4}\end{align*}$$
The calculation of the individual $i$’s choice of $x$ does not depend on
the numeraire in the first subsection, so I use this results here.
$$\begin{align*}
& m_1 + 2 = m_2 + 8 = m_3 + 18 = m_4 + 32\end{align*}$$ Initially, the
distribution of the numeraire was given by: $$\begin{align*}
m_1 = 10,\; m_2 = 20, \; m_3 = 30,\; m_4 = 40 \end{align*}$$ Now
endowments have to be changed so that the condition in equation (1)
holds: $$\begin{align*}
m^n_1 = 38,\; m^n_2 = 32, \; m^n_3 = 22,\; m^n_4 = 8 \end{align*}$$
Then, the amount of taxes is just the difference between the initial
$m_i$ and the nash bargaining $m^n_i$: 
$$\begin{align*}
tax_1 = m_1 - m_1^n = -28, \; tax_2 = m_2 - m_2^n = -12 , \\ tax_3 = m_3 - m_3^n = 8 \\
, \; tax_4 = m_4 - m_4^n = -32 \end{align*}$$ Negative taxes mean that
the individual obtains money and positives taxes mean that the
individual has to pay taxes.\
We than get $$\begin{align*}
W^n(u^n_i) = \Pi_{i=1}^4 (u^n_i)^{\alpha_i} = (m_1^n + 2)^{\alpha_1}(m_2^n + 8)^{\alpha_2}(m_3^n + 18)^{\alpha_3}(m_4^n + 32)^{\alpha_4} = 40 > 37.44\end{align*}$$

-----
Partial derivatives of the expenditure function with respect to prices\
$$\begin{align*}
&h_{1}(p,u) = \frac{{\partial}e(p,w)}{{\partial}{p_{1}}} = \frac{u}{2} \\
&h_{2}(p,u) = \frac{{\partial}e(p,w)}{{\partial}{p_{2}}} = u \\
&\rightarrow  h(p,u) = \left(\begin{array}{c}  \frac{u}{2} \\ u \end{array} \right)\end{align*}$$


![*Notes:* The survivor function does not go to zero by the end of the
time frame. This is due to censoring at the right. Some people still did
not find a new job.](gr_1 "Headline1"){width="90.00000%"}

![*Notes:* And since it makes fun, I will add one more, with a different width](gr_2 "Headline 2"){width="50.00000%"}

![A nice figure](https://github.com/jaschwer/assignment2/blob/gh-pages/gr_1.pdf)

![A nice figure](https://github.com/jaschwer/assignment2/blob/gh-pages/gr_1.png)

![A nice woooooow meme](http://pl.memgenerator.pl/mem-image/wooooooow-pl-ffffff-2)


